

Assignment #9

Hugo SALOU

1) We will write $P(x)$ (resp. $Q(x)$) for $\Pr_{x \sim P}[X=x]$ (resp. $\Pr_{x \sim Q}[X=x]$).

Here is the algorithm distinguishing P and Q :

for an input $x \in R$,

- if $P(x) > Q(x)$ then output " $P!$ "
- otherwise output " $Q!$ ".

We have the following lemma:

$$\max(a, b) = \frac{a+b}{2} + \frac{|a-b|}{2} \quad \text{when } a, b \geq 0$$

(if $a \geq b$, then $\frac{a+b}{2} + \frac{a-b}{2} = a$ and symmetrically for $b \geq a$).

$$\Pr[\text{success}] = \frac{1}{2} \cdot \Pr_{x \sim P}[P(x) > Q(x)] + \frac{1}{2} \Pr_{x \sim Q}[P(x) \leq Q(x)]$$

$$= \frac{1}{2} \sum_{\substack{x \in R \\ P(x) > Q(x)}} P(x) + \frac{1}{2} \sum_{\substack{x \in R \\ P(x) \leq Q(x)}} Q(x)$$

$$= \frac{1}{2} \sum_{x \in R} \max(P(x), Q(x))$$

$$= \frac{1}{2} \sum_{x \in R} \frac{P(x) + Q(x)}{2} + \frac{1}{2} \sum_{x \in R} \frac{|P(x) - Q(x)|}{2}$$

$$\underbrace{\sum_{x \in R} P(x) = \sum_{x \in R} Q(x) = 1}_{\frac{1}{2} \Delta(P, Q)}$$

$$= \frac{1}{2} + \frac{1}{2} \Delta(P, Q)$$

So, this algorithm distinguishes between P and Q with a success probability of $\frac{1}{2} + \frac{1}{2} \Delta(P, Q)$.

2) Let $p(x)$ be the probability that a distinguisher A between P and Q outputs "P!" on the input $x \in R$.

$$\begin{aligned}
 \Pr[\text{success}] &= \frac{1}{2} \Pr_{x \sim P}[A \text{ outputs "P!"}] + \frac{1}{2} \Pr_{x \sim Q}[A \text{ outputs "P!"}] \\
 &= \frac{1}{2} \sum_{x \in R} p(x) P(x) + \frac{1}{2} \sum_{x \in R} (1 - p(x)) Q(x) \\
 &= \frac{1}{2} \sum_{x \in R} (Q(x) + p(x) (P(x) - Q(x))) \\
 &= \frac{1}{2} + \frac{1}{2} \sum_{x \in R} p(x) (P(x) - Q(x)) \\
 &\leq \frac{1}{2} + \frac{1}{2} \sum_{x \in R} \max(0, P(x) - Q(x)) \\
 &\quad \text{as } p(x) \in [0, 1].
 \end{aligned}$$

And, we have that

$$0 = \sum_{x \in R} P(x) - \sum_{x \in R} Q(x) = \sum_{x \in R} (P(x) - Q(x)) = \sum_{P(x) > Q(x)} (P(x) - Q(x)) + \sum_{P(x) < Q(x)} (P(x) - Q(x))$$

then

$$\begin{aligned}
 \sum_{P(x) > Q(x)} |P(x) - Q(x)| &= - \sum_{P(x) < Q(x)} (P(x) - Q(x)) = \sum_{P(x) < Q(x)} (Q(x) - P(x)) \\
 &= \sum_{P(x) < Q(x)} |P(x) - Q(x)|
 \end{aligned}$$

thus

$$\begin{aligned}\sum_{x \in R} |P(x) - Q(x)| &= \sum_{P(x) > Q(x)} |P(x) - Q(x)| + \sum_{P(x) < Q(x)} |P(x) - Q(x)| \\ &= 2 \cdot \sum_{P(x) > Q(x)} (P(x) - Q(x)) \\ &= 2 \cdot \sum_{x \in R} \max(0, P(x) - Q(x))\end{aligned}$$

and we can conclude that

$$\begin{aligned}P[\text{success}] &\leq \frac{1}{2} + \frac{1}{2} \sum_{x \in R} \max(0, P(x) - Q(x)) \\ &\leq \frac{1}{2} + \frac{1}{2} \times \frac{1}{2} \sum_{x \in R} |P(x) - Q(x)| \\ &\leq \frac{1}{2} + \frac{1}{2} \Delta(P, Q)\end{aligned}$$

and so the success probability of the algorithm from 1) is optimal.

End of Assignment # 9